src/Sound/Semantics/Omni.dfy
@@ -2,61 +2,115 @@ module Omni {
   import opened Defs
   export
     provides Defs, SeqLemma, SemNest, WP, SemCons, SeqFrameLemmaAll
-    reveals Sem, SeqSem, SeqWP
+    reveals Sem, SeqSem, SeqWP, Continuation, Continuation.LessThan, Continuation.Update, Continuation.Delete
 
-  least predicate Sem(s: Stmt, st: State, post: iset<State>) {
-    match s
-    case Check(e)       => e.IsDefinedOn(st.Keys) && (st.Eval(e) &&  st in post)
-    case Assume(e)      => e.IsDefinedOn(st.Keys) && (st.Eval(e) ==> st in post)
-    case Seq(ss)        => SeqSem(ss, st, post)
-    case Assign(x, v)   => v.IsDefinedOn(st.Keys) && st.Update(x, st.Eval(v)) in post
-    case VarDecl(v, s)  => forall b: Value :: Sem(s, st.Update(v, b), UpdateSet(v, post))
-    case Choice(s0, s1) => Sem(s0, st, post) && Sem(s1, st, post)
-  }
+  newtype Continuation = map<Label, iset<State>> {
+    predicate LessThan(cont: Continuation) {
+      && Keys <= cont.Keys
+      && forall lbl <- Keys :: this[lbl] <= cont[lbl]
+    }
 
-  ghost function WP(s: Stmt, post: iset<State>) : iset<State> {
-    iset st: State | Sem(s, st, post)
-  }
+    ghost function Update(v: Variable) : Continuation {
+      map lbl | lbl in Keys :: UpdateSet(v, this[lbl])
+    }
 
-  least predicate SeqSem(ss: seq<Stmt>, st: State, post: iset<State>) {
-    if ss == [] then st in post else
-    forall post': iset<State> :: 
-      (forall st: State :: SeqSem(ss[1..], st, post) ==> st in post') ==> Sem(ss[0], st, post')
-  }
-
-  ghost function SeqWP(ss: seq<Stmt>, post: iset<State>): iset<State> {
-    iset st: State | SeqSem(ss, st, post)
-  }
-
-  least lemma SemCons(s: Stmt, st: State, post: iset<State>, post': iset<State>)
-    requires Sem(s, st, post)
-    requires post <= post'
-    ensures Sem(s, st, post')
-  {
-    match s
-    case VarDecl(v, s) => assert UpdateSet(v, post) <= UpdateSet(v, post');
-    case Seq(ss) => SeqSemCons(ss, st, post, post');
-    case _ =>
-  }
-
-  lemma SeqSemCons(ss: seq<Stmt>, st: State, post: iset<State>, post': iset<State>)
-    requires SeqSem(ss, st, post)
-    requires post <= post'
-    ensures SeqSem(ss, st, post')
-  {  }
-
-  least lemma SemNest(s: Stmt, ss: seq<Stmt>, st: State, post: iset<State>) 
-    requires Sem(s, st, SeqWP(ss, post))
-    ensures SeqSem([s] + ss, st, post)
-  {
-    forall post': iset<State> | SeqWP(ss, post) <= post' {
-      SemCons(s, st, SeqWP(ss, post), post');
+    ghost function Delete(v: Variable) : Continuation {
+      map lbl | lbl in Keys :: DeleteSet(v, this[lbl])
     }
   }
 
-  lemma SeqSemNest(ss1: seq<Stmt>, ss2: seq<Stmt>, st: State, post: iset<State>) 
-    requires SeqSem(ss1 + ss2, st, post)
-    ensures SeqSem(ss1, st, SeqWP(ss2, post))
+  /**
+    (l :: var y; exit l); y := 0
+    wp ((l :: var y; exit l); y := 0, True, {}) == 
+    wp ((l ::var y; exit l), wp(y := 0, True, {}), {}) == 
+    wp ((l ::var y; exit l), fun st => y in st, {}) == 
+    wp ((var y; exit l), fun st => y in st, {l |-> fun st => y in st}) == 
+    fun st => forall b: bool, wp ((exit l), False, {l |-> fun st => y in st}) st[y := b]
+    fun st => forall b: bool, y in st[y := b]
+   */
+
+  least predicate Sem(s: Stmt, st: State, post: iset<State>, cont: Continuation) {
+    match s
+    case Check(e)            => e.IsDefinedOn(st.Keys) && (st.Eval(e) &&  st in post)
+    case Assume(e)           => e.IsDefinedOn(st.Keys) && (st.Eval(e) ==> st in post)
+    case Seq(ss)             => SeqSem(ss, st, post, cont)
+    case Assign(x, v)        => 
+      && x in st
+      && v.IsDefinedOn(st.Keys) 
+      && st.Update(x, st.Eval(v)) in post
+    case VarDecl(v, s)       => forall b: Value :: Sem(s, st.Update(v, b), UpdateSet(v, post), cont.Update(v))
+    case Choice(s0, s1)      => Sem(s0, st, post, cont) && Sem(s1, st, post, cont)
+    case LabeledStmt(lbl, s) => Sem(s, st, post, cont[lbl := post])
+    case Exit(lbl)           => lbl in cont && st in cont[lbl]
+  }
+
+  ghost function WP(s: Stmt, post: iset<State>, cont: Continuation) : iset<State> {
+    iset st: State | Sem(s, st, post, cont)
+  }
+
+  least predicate SeqSem(ss: seq<Stmt>, st: State, post: iset<State>, cont: Continuation) {
+    if ss == [] then st in post else
+    forall post': iset<State> :: 
+      (forall st: State :: SeqSem(ss[1..], st, post, cont) ==> st in post') ==> Sem(ss[0], st, post', cont)
+  }
+
+  ghost function SeqWP(ss: seq<Stmt>, post: iset<State>, cont: Continuation): iset<State> {
+    iset st: State | SeqSem(ss, st, post, cont)
+  }
+
+  lemma SemConsCont(s: Stmt, st: State, post: iset<State>, post': iset<State>, cont: Continuation, cont': Continuation)
+    requires Sem(s, st, post, cont)
+    requires post <= post'
+    requires cont.LessThan(cont')
+    ensures Sem(s, st, post', cont')
+  {
+    match s
+    case VarDecl(v, s) => 
+      assert cont.Update(v).LessThan(cont'.Update(v));
+      assert UpdateSet(v, post) <= UpdateSet(v, post');
+    case Seq(ss) => SeqSemConsCont(ss, st, post, post', cont, cont');
+    case LabeledStmt(lbl, s) => assert cont[lbl := post].LessThan(cont'[lbl := post']);
+    case _ =>
+  }
+
+  lemma SeqSemConsCont(ss: seq<Stmt>, st: State, post: iset<State>, post': iset<State>, cont: Continuation, cont': Continuation)
+    requires SeqSem(ss, st, post, cont)
+    requires post <= post'
+    requires cont.LessThan(cont')
+    ensures SeqSem(ss, st, post', cont')
+  {
+    if ss != [] {
+      forall post'': iset<State> | SeqWP(ss[1..], post', cont') <= post''
+        ensures Sem(ss[0], st, post'', cont') {
+        SemConsCont(ss[0], st, post'', post'', cont, cont');
+      }
+    }
+  }
+
+  least lemma SemCons(s: Stmt, st: State, post: iset<State>, post': iset<State>, cont: Continuation)
+    requires Sem(s, st, post, cont)
+    requires post <= post'
+    ensures Sem(s, st, post', cont)
+  { SemConsCont(s, st, post, post', cont, cont); }
+
+  lemma SeqSemCons(ss: seq<Stmt>, st: State, post: iset<State>, post': iset<State>, cont: Continuation)
+    requires SeqSem(ss, st, post, cont)
+    requires post <= post'
+    ensures SeqSem(ss, st, post', cont)
+  { SeqSemConsCont(ss, st, post, post', cont, cont); }
+
+  least lemma SemNest(s: Stmt, ss: seq<Stmt>, st: State, post: iset<State>, cont: Continuation) 
+    requires Sem(s, st, SeqWP(ss, post, cont), cont)
+    ensures SeqSem([s] + ss, st, post, cont)
+  {
+    forall post': iset<State> | SeqWP(ss, post, cont) <= post' {
+      SemCons(s, st, SeqWP(ss, post, cont), post', cont);
+    }
+  }
+
+  lemma SeqSemNest(ss1: seq<Stmt>, ss2: seq<Stmt>, st: State, post: iset<State>, cont: Continuation) 
+    requires SeqSem(ss1 + ss2, st, post, cont)
+    ensures SeqSem(ss1, st, SeqWP(ss2, post, cont), cont)
   {
     if ss1 == [] {
       assert [] + ss2 == ss2;
@@ -66,69 +120,74 @@ module Omni {
     }
   }
 
-  lemma SeqLemma(ss: seq<Stmt>, cont: seq<Stmt>, st: State, post: iset<State>)
-    requires Sem(Seq(ss + cont), st, post)
-    ensures SeqSem([Seq(ss)] + cont, st, post)
+  lemma SeqLemma(ss1: seq<Stmt>, ss2: seq<Stmt>, st: State, post: iset<State>, cont: Continuation)
+    requires Sem(Seq(ss1 + ss2), st, post, cont)
+    ensures SeqSem([Seq(ss1)] + ss2, st, post, cont)
   {
-    SeqSemNest(ss, cont, st, post);
-    SemNest(Seq(ss), cont, st, post);
+    SeqSemNest(ss1, ss2, st, post, cont);
+    SemNest(Seq(ss1), ss2, st, post, cont);
   }
 
-  lemma FrameLemma(s: Stmt, v: Variable, st: State, post: iset<State>)
-    requires Sem(s, st, post)
+  lemma FrameLemma(s: Stmt, v: Variable, st: State, post: iset<State>, cont: Continuation)
+    requires Sem(s, st, post, cont)
     requires v !in s.FVars()
     requires v !in s.BVars()
-    ensures Sem(s, st - {v}, DeleteSet(v, post))
+    ensures Sem(s, st - {v}, DeleteSet(v, post), cont.Delete(v))
   {
     match s 
     case Assign(x, e) => e.EvalFVarsLemma(st, st - {v});
     case Check(e) => e.EvalFVarsLemma(st, st - {v});
     case Assume(e) =>  e.EvalFVarsLemma(st, st - {v});
-    case Seq(ss) => SeqFrameLemma(ss, v, st, post);
+    case Seq(ss) => SeqFrameLemma(ss, v, st, post, cont);
     case VarDecl(u, s) =>
       forall c: Value {: trigger}
-        ensures Sem(s, (st - {v}).Update(u, c), UpdateSet(u, DeleteSet(v, post))) { 
-        FrameLemma(s, v, st.Update(u, c), UpdateSet(u, post));
+        ensures Sem(s, (st - {v}).Update(u, c), UpdateSet(u, DeleteSet(v, post)), cont.Delete(v).Update(u)) { 
+        FrameLemma(s, v, st.Update(u, c), UpdateSet(u, post), cont.Update(u));
         assert forall c :: (st - {v}).Update(u, c) == st.Update(u, c) - {v};        
-        SemCons(s, (st - {v}).Update(u, c), DeleteSet(v, UpdateSet(u, post)), UpdateSet(u, DeleteSet(v, post))) by {
-          forall st | st in DeleteSet(v, UpdateSet(u, post)) 
-            ensures st in UpdateSet(u, DeleteSet(v, post)) {
-            assert forall b :: (st - {u}).Update(v, b) == st.Update(v, b) - {u};
-          }
+        SemConsCont(s, (st - {v}).Update(u, c), 
+          DeleteSet(v, UpdateSet(u, post)), 
+          UpdateSet(u, DeleteSet(v, post)), 
+          cont.Update(u).Delete(v),
+          cont.Delete(v).Update(u)) by {
+          // forall st | st in DeleteSet(v, UpdateSet(u, post)) 
+          //   ensures st in UpdateSet(u, DeleteSet(v, post)) {
+          //   assert forall b :: (st - {u}).Update(v, b) == st.Update(v, b) - {u};
+          // }
         }
       }
-    case Choice(s0, s1) => FrameLemma(s0, v, st, post); FrameLemma(s1, v, st, post);
+    case Choice(s0, s1) => FrameLemma(s0, v, st, post, cont); FrameLemma(s1, v, st, post, cont);
+    case _ => assume {:axiom} false;
   }
 
-  lemma SeqFrameLemma(ss: seq<Stmt>, v: Variable, st: State, post: iset<State>)
-    requires SeqSem(ss, st, post)
+  lemma SeqFrameLemma(ss: seq<Stmt>, v: Variable, st: State, post: iset<State>, cont: Continuation)
+    requires SeqSem(ss, st, post, cont)
     requires v !in SeqBVars(ss)
     requires v !in SeqFVars(ss)
-    ensures SeqSem(ss, st - {v}, DeleteSet(v, post))
+    ensures SeqSem(ss, st - {v}, DeleteSet(v, post), cont.Delete(v))
   {
     if ss == [] {
     } else {
       assert ([ss[0]] + ss[1..])[0] == ss[0];
-      FrameLemma(ss[0], v, st, SeqWP(ss[1..], post));
-      SemNest(ss[0], ss[1..], st - {v}, DeleteSet(v, post)) by {
-        SemCons(ss[0], st - {v}, DeleteSet(v, SeqWP(ss[1..], post)), SeqWP(ss[1..], DeleteSet(v, post))) by {
-          forall st | st in DeleteSet(v, SeqWP(ss[1..], post)) 
-            ensures SeqSem(ss[1..], st, DeleteSet(v, post)) {
-            var st': State :| st == st' - {v} && SeqSem(ss[1..], st', post);
-            SeqFrameLemma(ss[1..], v, st', post);
+      FrameLemma(ss[0], v, st, SeqWP(ss[1..], post, cont), cont);
+      SemNest(ss[0], ss[1..], st - {v}, DeleteSet(v, post), cont.Delete(v)) by {
+        SemCons(ss[0], st - {v}, DeleteSet(v, SeqWP(ss[1..], post, cont)), SeqWP(ss[1..], DeleteSet(v, post), cont.Delete(v)), cont.Delete(v)) by {
+          forall st | st in DeleteSet(v, SeqWP(ss[1..], post, cont)) 
+            ensures SeqSem(ss[1..], st, DeleteSet(v, post), cont.Delete(v)) {
+            var st': State :| st == st' - {v} && SeqSem(ss[1..], st', post, cont);
+            SeqFrameLemma(ss[1..], v, st', post, cont);
           }
         }
       }
     }
   }
 
-  lemma SeqFrameLemmaAll(ss: seq<Stmt>, v: Variable, st: State)
-    requires SeqSem(ss, st, AllStates)
+  lemma SeqFrameLemmaAll(ss: seq<Stmt>, v: Variable, st: State, cont: Continuation)
+    requires SeqSem(ss, st, AllStates, cont)
     requires v !in SeqBVars(ss)
     requires v !in SeqFVars(ss)
-    ensures SeqSem(ss, st - {v}, AllStates)
+    ensures SeqSem(ss, st - {v}, AllStates, cont.Delete(v))
   {
-    SeqFrameLemma(ss, v, st, AllStates);
-    SeqSemCons(ss, st - {v}, DeleteSet(v, AllStates), AllStates);
+    SeqFrameLemma(ss, v, st, AllStates, cont);
+    SeqSemCons(ss, st - {v}, DeleteSet(v, AllStates), AllStates, cont.Delete(v));
   }
 }
